FormalWeb.lean
@@ -1,11 +1,14 @@
 -- This module serves as the root of the `FormalWeb` library.
 -- Import modules here that should be built as part of the library.
 import FormalWeb.Document
+import FormalWeb.EventLoop
+import FormalWeb.EventLoopMessage
 import FormalWeb.FFI
 import FormalWeb.SessionHistory
 import FormalWeb.Navigation
 import FormalWeb.TransitionTrace
 import FormalWeb.Fetch
+import FormalWeb.Proofs.EventLoopProof
 import FormalWeb.Proofs.FetchProof
 import FormalWeb.Proofs.UserAgentProof
 import FormalWeb.Traversable
